---
title: "Maximum Likelihood Estimation"
output:
  html_document:
    df_print: paged
---

This is a notebook to show how the coefficients for logit are derived

$\begin{aligned}
P(y|\beta) = P(y_1, y_2,...,y_n|\beta) = \prod_{y=1}P(y_{i}=1)^{y} \times \prod_{y=0}(1-P(y_{i}=1))^{1-y}
\end{aligned}$

Assume $P(y)$ is predicted using a logistic function, in this case termed:

$P(y|\beta)=\Lambda(X'\beta)=(1+e^{-X'\beta})^{-1}$

Then we can use the log likelihood to change from product to sum:

$\begin{aligned}
& = \prod_{y=1} \Lambda(X'\beta)^{y} \times \prod_{y=0}(1-X'\beta)^{1-y} \\
& = \sum{\text{log}(\Lambda(X'\beta)^{y})} + \sum{\text{log}(\Lambda(1-X'\beta)^{1-y})} \\
& = \sum_{i=1}^{n}{y\text{log}(\Lambda(X'\beta)) + (1-y)\text{log}(\Lambda(1-X'\beta))}
\end{aligned}$

Which as a sum is now easier to differentiate to get the coefficients:

$\begin{aligned}
& \leftrightarrow \frac{\partial}{\partial\beta_j}P(y|\beta) \\
& = \frac{\partial}{\partial\beta_j}\sum{y\text{log}(\Lambda(X'\beta)) + (1-y)\text{log}(\Lambda(1-X'\beta))} \\
& =\sum_{i=1}^{n}{y\frac{\frac{\partial}{\partial\beta_j}\Lambda(X'\beta)}{\Lambda(X'\beta)} + (1-y)\frac{\frac{\partial}{\partial\beta_j}\Lambda(X'\beta)}{\Lambda(X'\beta)}}
\end{aligned}$

Which you can simplify in the following way using the logistic function:



$\begin{aligned}
& = \frac{\partial}{\partial\beta_j}\Lambda(X'\beta) \\
& = \frac{\partial}{\partial\beta_j}(1+e^{-X'\beta})^{-1} \\
& = -1(1+e^{-X'\beta})^{-2} \times -x_je^{-X\beta} \\
& = x_j\left[\frac{e^{-X\beta}}{(1+e^{-X'\beta})^{2}}\right] \\
& = x_{j}\left[\frac{1}{1+e^{-X'\beta}} \times \frac{e^{-X\beta}}{1+e^{-X'\beta}}\right] \\
& = x_{j}\left[\frac{1}{1+e^{-X'\beta}} \times \left(1-\frac{1}{1+e^{-X'\beta}}\right)\right] \\
& = x_{j}\left[\Lambda(X'\beta)\times\left(1-\Lambda(X'\beta)\right)\right]
\end{aligned}$

And hence derive the optimal maximum log-likelihood coefficient:

$\begin{aligned}
& \leftrightarrow	\frac{\partial}{\partial\beta_j}P(y|\beta) \\
& =\sum_{i=1}^{n}{y\frac{\frac{\partial}{\partial\beta_j}\Lambda(X'\beta)}{\Lambda(X'\beta)}} \\
& =\sum_{i=1}^{n}{y\frac{x_{j}\left[\Lambda(X'\beta)\times\left(1-\Lambda(X'\beta)\right)\right]}{\Lambda(X'\beta)} + 
(1-y)\frac{x_{j}\left[\Lambda(X'\beta)\times\left(1-\Lambda(X'\beta)\right)\right]}{1-\Lambda(X'\beta)} 
} \\
& =\sum_{i=1}^{n}{x_{j}\left[y\left(1-\Lambda(X'\beta)\right) + (1-y)\left(\Lambda(X'\beta)\right)\right]}
\end{aligned}$


